clight_examples/xorlist/xorlist01proof.v
@@ -12,10 +12,12 @@ Require Import HTactics ProofMode.
 Require Import HSim IProofMode.
 Require Import ClightDmgen.
 Require Import ClightDmMem1.
+Require Import CIProofMode.
 Require Import xorlist.
 Require Import xorlist0.
 Require Import xorlist1.
 Require Import CTactics.
+(* Require Import Int64Arith. *)
 (* Require Import ClightProofs.
 Require Import csyntax.
 Require Import ClightPreambles. *)
@@ -77,9 +79,48 @@ Section PROOF.
     - apply sim_encrypt.
   Qed. *)
   Arguments alist_add /.
-  Arguments ccallU /.
 
   Let ce := map (fun '(id, p) => (string_of_ident id, p)) (Maps.PTree.elements (prog_comp_env prog)).
+
+  Lemma ptrofs_max : Archi.ptr64 = true -> Int64.max_unsigned = Ptrofs.max_unsigned.
+  Proof. des_ifs_safe. Qed.
+  
+  Lemma mkint64_eq' x y : Int64.unsigned x = Int64.unsigned y -> x = y.
+  Proof. i. destruct x. destruct y. apply Int64.mkint_eq. et. Qed.
+
+  Lemma lxor_size a b
+    :
+  0 ≤ a ≤ Ptrofs.max_unsigned
+  -> 0 ≤ b ≤ Ptrofs.max_unsigned
+  -> 0 ≤ Z.lxor a b ≤ Ptrofs.max_unsigned.
+  Proof.
+    i. change Ptrofs.max_unsigned with (2 ^ 64 - 1) in *.
+    assert (I1: 0 ≤ a < 2 ^ 64) by nia.
+    assert (I2: 0 ≤ b < 2 ^ 64) by nia. clear H3 H4.
+    assert (0 ≤ Z.lxor a b < 2 ^ 64); try nia.
+    destruct (Coqlib.zeq a 0);
+    destruct (Coqlib.zeq b 0); clarify.
+    2: split.
+    - rewrite Z.lxor_0_r. nia.
+    - rewrite Z.lxor_nonneg. nia.
+    - des.
+      rewrite Z.log2_lt_pow2 in I3; try nia.
+      rewrite Z.log2_lt_pow2 in I0; try nia.
+      destruct (Coqlib.zeq (Z.lxor a b) 0); try nia.
+      rewrite Z.log2_lt_pow2; cycle 1.
+      + assert (0 ≤ Z.lxor a b); try nia. rewrite Z.lxor_nonneg. nia.
+      + eapply Z.le_lt_trans; try apply Z.log2_lxor; try nia. 
+  Qed.
+
+Arguments ClightDmExprgen.sem_xor_c /.
+Arguments ClightDmExprgen.sem_binarith_c /.
+Arguments ClightDmExprgen.sem_cast_c /.
+
+Create HintDb ptrArith.
+
+Hint Unfold Vptrofs Int64.xor Ptrofs.to_int64 : ptrArith.
+Hint Rewrite ptrofs_max Ptrofs.unsigned_repr Int64.unsigned_repr : ptrArith.
+Hint Resolve Ptrofs.unsigned_range_2 : ptrArith.
 
   Lemma val_multimap v b ofs : (v ⊸ (b, ofs)) -∗ ⌜exists i, v = Vptrofs i \/ exists b ofs, v = Vptr b ofs⌝.
   Proof.
@@ -94,6 +135,19 @@ Section PROOF.
     -∗ b ↱q0# (z, t, Some (Ptrofs.unsigned i)).
   Proof. Admitted.
 
+  Lemma add_provenance b ofs q sz tg i i'
+    :
+  b ↱q# (sz, tg, Some i) ** Vptrofs i' ⊸ (b, ofs) -∗ ⌜(i + ofs)%Z = Ptrofs.unsigned i'⌝.
+  Proof. 
+    iIntros "[BLK PTR]". unfold allocated_with, repr_to. des_ifs.
+    iDestruct "BLK" as "[ALLOC [BL PTR']]".
+    iCombine "PTR" "PTR'" as "PTR".
+    iPoseProof (provenace_dup with "PTR") as "%". clarify.
+    iPureIntro.
+    unfold Vptrofs in *. des_ifs_safe. unfold Ptrofs.to_int64.
+    do 2 autorewrite with ptrArith; auto with ptrArith. nia.
+  Qed.
+
   Lemma sim_encrypt (sk: Sk.t) :
     sim_fnsem wf top2
       ("encrypt", fun_to_tgt "xorlist" (GlobalStb sk) (mk_pure encrypt_spec))
@@ -102,262 +156,357 @@ Section PROOF.
     Opaque repr_to.
     Opaque allocated_with.
     Opaque points_to.
-    Opaque Maps.PTree.set.
-    Opaque Maps.PTree.get.
+    Opaque ccallU.
     econs; ss. red.
     apply isim_fun_to_tgt; auto. i; ss.
     unfold decomp_func, function_entry_c. ss.
     iIntros "[INV PRE]". des_ifs_safe. ss.
     iDestruct "PRE" as "[PRE %]".
-    iDestruct "PRE" as (ofs1 ofs2 opt1 opt2) "[[[[% PTR1] ARG1] PTR2] ARG2]".
+    iDestruct "PRE" as (opt1 opt2) "[[[[% PTR1] ARG1] PTR2] ARG2]".
     ss. clarify. hred_r. iApply isim_tau_tgt. hred_r. iApply isim_tau_tgt.
     ss. hred_r. des_ifs_safe.
-    iApply isim_apc. iExists (Some (2 : Ord.t)).
+    iApply isim_apc. iExists (Some (2%nat : Ord.t)).
     iPoseProof (val_multimap with "PTR1") as "%".
     iPoseProof (val_multimap with "PTR2") as "%".
     des.
-    - unfold Vptrofs in *; des_ifs_safe. hred_r.
-      iApply isim_call_pure.
-      { eapply fn_has_spec_in_stb.
-        { eapply MEMINCL. stb_tac. ss. }
-        { oauto. }
-        { ss. } }
-      { oauto. }
-      iSplitL "INV".
-      { iSplitL "INV"; auto. ss.
-        iSplits; ss. instantiate (1:=True%I); et. }
-      iIntros (st_src0 st_tgt0 ret_src ret_tgt) "[INV POST]".
-      ss. iDestruct "POST" as "[% %]". ss. clarify.
+    - des_ifs. hred_r. rewrite <- Heq.
+      iApply isim_ccallU_capture1; ss; oauto.
+      iSplitL "INV"; iFrame.
+      iIntros (st_src0 st_tgt0) "INV".
       hred_r. iApply isim_tau_tgt. hred_r. iApply isim_tau_tgt.
       hred_r. iApply isim_tau_tgt. ss. hred_r.
-      iApply isim_call_pure.
-      { eapply fn_has_spec_in_stb.
-        { eapply MEMINCL. stb_tac. ss. }
-        { oauto. }
-        { ss. } }
-      { oauto. }
-      iSplitL "INV".
-      { iSplitL "INV"; auto. ss.
-        iSplits; ss. instantiate (1:=True%I); et. }
-      iIntros (st_src1 st_tgt1 ret_src ret_tgt) "[INV POST]".
-      ss. iDestruct "POST" as "[% %]". ss. clarify.
-      hred_r. iApply isim_tau_tgt. hred_r. iApply isim_tau_tgt. ss.
-      hred_r.
-      unfold ClightDmExprgen.sem_xor_c, ClightDmExprgen.sem_binarith_c, ClightDmExprgen.sem_cast_c.
-      ss. des_ifs_safe. hred_r. hred_l. iApply isim_choose_src. iExists _.
+      des_ifs. hred_r. rewrite <- Heq2.
+      iApply isim_ccallU_capture1; ss; oauto.
+      iSplitL "INV"; iFrame.
+      iIntros (st_src1 st_tgt1) "INV".
+      hred_r. iApply isim_tau_tgt. hred_r. iApply isim_tau_tgt.
+      ss. hred_r.
+      des_ifs_safe. hred_r. hred_l. iApply isim_choose_src. iExists _.
       iApply isim_ret. iSplits; ss.
-      iSplitR "ARG2". 
-      iSplitR "ARG1".
-      {  } 
+      admit.
+      (* iSplitR "ARG2 PTR2". 
+      iSplitR "ARG1 PTR1".
+      { iPureIntro. f_equal.
+        instantiate (1:=Ptrofs.unsigned i0).
+        instantiate (1:=Ptrofs.unsigned i).
+        autounfold with ptrArith in *. des_ifs_safe. f_equal.
+        autorewrite with ptrArith.
+        4:{ autorewrite with asdf; ss. auto with asdf. }
+        3:{ autorewrite with asdf; ss. auto with asdf. }
+        2:{ apply lxor_size; auto with asdf. }
+        { f_equal. apply Z.lxor_comm. } }
+      { admit. }
+      { admit. } *)
+    - des_ifs_safe. hred_r. iApply isim_ccallU_capture2; ss; oauto.
+      iSplitL "INV ARG1 PTR1". { admit. }
+      iIntros (st_src0 st_tgt0 ret) "[INV POST]".
+      iDestruct "POST" as (i1) "[% POST]".
+      clarify. hred_r. iApply isim_tau_tgt.
+      hred_r. iApply isim_tau_tgt. hred_r.
+      iApply isim_tau_tgt. ss. hred_r. des_ifs_safe.
+      hred_r. rewrite <- Heq. iApply isim_ccallU_capture1; ss; oauto.
+      iSplitL "INV"; ss. iIntros (st_src1 st_tgt1) "INV".
+      hred_r. iApply isim_tau_tgt. hred_r.
+      iApply isim_tau_tgt. ss. hred_r. des_ifs_safe.
+      hred_r. hred_l. iApply isim_choose_src. iExists _.
+      iApply isim_ret. iSplits; ss.
+      admit.
+    - des_ifs_safe. hred_r. rewrite <- Heq. iApply isim_ccallU_capture1; ss; oauto.
+      iSplitL "INV"; ss. iIntros (st_src1 st_tgt1) "INV".
+      hred_r. iApply isim_tau_tgt. hred_r.
+      iApply isim_tau_tgt. ss. hred_r. iApply isim_tau_tgt.
+      hred_r. des_ifs_safe. hred_r.
+      iApply isim_ccallU_capture2; ss; oauto.
+      iSplitL "INV ARG1 PTR1". { admit. }
+      iIntros (st_src0 st_tgt0 ret) "[INV POST]".
+      iDestruct "POST" as (i2) "[% POST]".
+      clarify. hred_r. iApply isim_tau_tgt.
+      hred_r. iApply isim_tau_tgt. ss. hred_r.
+      des_ifs_safe. hred_r.
+      hred_l. iApply isim_choose_src. iExists _.
+      iApply isim_ret. iSplits; ss.
+      admit.
+    - des_ifs_safe. hred_r. iApply isim_ccallU_capture2; ss; oauto.
+      iSplitL "INV PTR1 ARG1". { admit. }
+      iIntros (st_src0 st_tgt0 ret) "[INV POST]".
+      iDestruct "POST" as (i1) "[% LIV]".
+      hred_r. iApply isim_tau_tgt. hred_r. iApply isim_tau_tgt.
+      hred_r. iApply isim_tau_tgt. ss. hred_r.
+      iApply isim_ccallU_capture2; ss; oauto.
+      iSplitL "INV PTR2 ARG2". { admit. }
+      iIntros (st_src1 st_tgt1 ret0) "[INV POST]".
+      iDestruct "POST" as (i2) "[% LIV1]".
+      hred_r. iApply isim_tau_tgt. hred_r. iApply isim_tau_tgt.
+      hred_r. ss. hred_r. des_ifs_safe. hred_r.
+      hred_l. iApply isim_choose_src. iExists _.
+      iApply isim_ret. iSplits; ss.
+      admit.
+    Unshelve. all: et. 
+  Admitted.
 
-
-
-      
-      iSplitL "-"; auto.
-      acatch. { apply MEMINCL. stb_tac. auto. } steps.
-      hcall (fun vret => ⌜vret = (Vlong (Ptrofs.to_int64 i0))↑⌝%I) _ with "".
-      { iModIntro. iSplits; ss. instantiate (1:=True%I). et. }
-      { oauto. }
-      mDesAll. des. subst. steps.
-      acatch. { apply MEMINCL. stb_tac. auto. }
-      steps.
-      hcall (fun vret => ⌜vret = (Vlong (Ptrofs.to_int64 i))↑⌝%I) _ with "".
-      { iModIntro. iSplits; ss. instantiate (1:=True%I). et. }
-      { oauto. }
-      mDesAll. des. subst. steps.
-      unfold ClightDmExprgen.sem_xor_c, ClightDmExprgen.sem_binarith_c, ClightDmExprgen.sem_cast_c.
-      steps. astop. steps. force_l. eexists. steps. hret tt; ss.
-      iModIntro. iSplits; ss.
-      iSplitR "A A1". iSplitR "A3 A2".
-      all: cycle 1.
-      { iApply val_exists. iFrame. }
-      { iApply val_exists. iFrame. }
-      iPureIntro. repeat f_equal. admit.
-    - unfold Vptrofs in *; des_ifs_safe. steps.
-      acatch. { apply MEMINCL. stb_tac. auto. } steps.
-      hcall _ _ with "".
-      { iModIntro. iSplits; ss.
-        { unfold capture_resource. iPureIntro. eexists _, _, _.
-          et. }
-       instantiate (1:=True%I). et. }
-      { oauto. }
-      mDesAll. des. subst. steps.
-
-     admit.
-    - unfold Vptrofs in *; des_ifs_safe. steps. admit.
-    - steps. admit.
-    mDesAll.
-    des_ifs; ss; des_ifs_safe; mDesAll; try solve [inv PURE]; steps.
-    - 
-    unfold alist_add. ss. alist_remove. ss.
-    repeat (rewrite decomp_seq); steps.
-    destruct build_composite_env'. steps. 
-    steps. unfold function_entry_c. steps. resolve_seq. 
-    unfold is_valid_ptr in ACC. 
-    destruct v1;destruct v2;mDesAll;ss;steps.
-    - rewrite decomp_builtin. ss. resolve_var.
-      resolve_seq.
-      rewrite decomp_builtin. ss. resolve_var.
-      rewrite decomp_ret. unfold _sreturn_c. steps. resolve_get. resolve_get. steps.
-      unfold sem_xor_c, sem_binarith_c, sem_cast_c. steps. astop. steps. force_l. eexists. steps.
-      hret tt;ss. iModIntro. iSplit;ss. iSplit;ss.
-      iExists (Ptrofs.of_int64 i), (Ptrofs.of_int64 i0).
-      iSplits;unfold Vptrofs in *;des_ifs_safe;repeat (rewrite Ptrofs.of_int64_to_int64;ss).
-      unfold Vnullptr in *. des_ifs_safe.
-    - rewrite decomp_builtin. ss. resolve_var.
-      resolve_seq.
-      rewrite decomp_builtin. ss. resolve_var.
-      astart 1. unfold ccallU. steps. acatch. { apply MEMINCL. stb_tac. auto. }
-      hcall (_, _) _ with "".
-      { iModIntro. iSplits;ss. }
-      { oauto. } mDesAll. des.
-      steps.
-      rewrite decomp_ret. unfold _sreturn_c. steps. resolve_get. resolve_get. steps.
-      unfold sem_xor_c, sem_binarith_c, sem_cast_c. steps. astop. steps. force_l. eexists. steps.
-      hret tt;ss. iModIntro. iSplit;ss. iSplit;ss.
-      iExists (Ptrofs.of_int64 i), (Ptrofs.of_int64 i1).
-      iSplitR "A1";[iSplitL "POST";[iSplitR "POST";[iSplits|]|auto]|];unfold Vptrofs in *;des_ifs_safe;repeat (rewrite Ptrofs.of_int64_to_int64;ss).
-      + unfold Vnullptr in *. des_ifs_safe.
-      + iExists _, _. iSplits;[..|iApply "POST"];ss.
-      + iExists _. iSplits;ss.
-    - rewrite decomp_builtin. ss. resolve_var.
-      astart 1. unfold ccallU. steps. acatch. { apply MEMINCL. stb_tac. auto. }
-      hcall (_, _) _ with "".
-      { iModIntro. iSplits;ss. }
-      { oauto. } mDesAll. des.
-      unfold ccallU. steps. resolve_seq.
-      rewrite decomp_builtin. ss. resolve_var.
-      rewrite decomp_ret. unfold _sreturn_c. steps. resolve_get. resolve_get. steps.
-      unfold sem_xor_c, sem_binarith_c, sem_cast_c. steps. astop. steps. force_l. eexists. steps.
-      hret tt;ss. iModIntro. iSplit;ss. iSplit;ss.
-      iExists (Ptrofs.of_int64 i1), (Ptrofs.of_int64 i0).
-      iSplits;ss.
-      iSplitR "A2";[iSplits;ss|];unfold Vptrofs in *;des_ifs_safe;repeat (rewrite Ptrofs.of_int64_to_int64;ss).
-      + rewrite Int64.xor_commut. rewrite Ptrofs.xor_commut. unfold Vnullptr in *. des_ifs_safe.
-      + iExists _. iSplits;ss.
-    - rewrite decomp_builtin. ss. resolve_var.
-      astart 2. unfold ccallU. steps. acatch. { apply MEMINCL. stb_tac. auto. }
-      hcall (_, _) _ with "".
-      { iModIntro. iSplits;ss. }
-      { oauto. } mDesAll. des.
-      steps. resolve_seq.
-      rewrite decomp_builtin. ss. resolve_var.
-      unfold ccallU. steps. acatch. { apply MEMINCL. stb_tac. auto. }
-      hcall (_, _) _ with "".
-      { iModIntro. iSplit;ss. }
-      { oauto. } mDesAll. des.
-      steps.
-      rewrite decomp_ret. unfold _sreturn_c. steps. resolve_get. resolve_get. steps.
-      unfold sem_xor_c, sem_binarith_c, sem_cast_c. steps. astop. steps. force_l. eexists. steps.
-      hret tt;ss. iModIntro. iSplit;ss. iSplit;ss.
-      iExists (Ptrofs.of_int64 i2), (Ptrofs.of_int64 i1).
-      iSplitR "A1";[iSplitR "A2";[iSplitR "POST1";[iSplitR "POST"|]|]|];unfold Vptrofs in *;des_ifs_safe;repeat (rewrite Ptrofs.of_int64_to_int64;ss).
-      + unfold Int64.xor, Ptrofs.xor. iPureIntro. f_equal. f_equal. unfold Ptrofs.to_int64. f_equal.
-        do 2 rewrite Int64.unsigned_repr_eq. rewrite Ptrofs.unsigned_repr_eq.
-        replace Ptrofs.modulus with Int64.modulus by auto.
-        set (Ptrofs.unsigned (Ptrofs.add i a)) as x. set (Ptrofs.unsigned (Ptrofs.add i0 a2)) as y.
-        admit "".
-      + iExists _, _. iSplits;[..|iApply "POST"];ss.
-      + iExists _, _. iSplits;[..|iApply "POST1"];ss.
-      + iExists _. iSplits;ss.
-      + iExists _. iSplits;ss.
-        Unshelve. all: et. 
-  Qed.
-
-  Lemma sim_decrypt (sk: alist string Sk.gdef) :
+  Lemma sim_decrypt (sk: Sk.t) :
     sim_fnsem wf top2
-      ("decrypt",
-        fun_to_tgt (SModSem.mn (SMod.get_modsem Sxor sk)) (GlobalStb sk)
-                   {| fsb_fspec := decrypt_spec; fsb_body := λ _ : option string * Any.t, triggerNB |})
-      ("decrypt", cfunU decrypt_body).
+      ("decrypt", fun_to_tgt "xorlist" (GlobalStb sk) (mk_pure decrypt_spec))
+      ("decrypt", cfunU (decomp_func sk ce f_decrypt)).
   Proof.
-    init. harg. destruct x. destruct p as [v1 v2]. mDesAll. des.
-    steps. unfold function_entry_c. steps. resolve_seq. 
-    unfold is_valid_ptr in ACC. 
-    destruct v2;mDesAll;ss;steps.
-    - rewrite decomp_builtin. ss. resolve_var.
-      rewrite decomp_ret. unfold _sreturn_c. steps. resolve_get. resolve_get. steps.
-      unfold sem_xor_c, sem_binarith_c, sem_cast_c. steps. astop. steps. force_l. eexists. steps.
-      hret tt;ss. iModIntro. iSplit;ss. iSplit;ss.
-      iExists (Ptrofs.of_int64 i).
-      iSplits;ss. rewrite Int64.xor_commut. rewrite Ptrofs.xor_commut.
-      unfold Vptrofs, Vnullptr in *;des_ifs_safe. 
-    - rewrite decomp_builtin. ss. resolve_var.
-      astart 2. unfold ccallU. steps. acatch. { apply MEMINCL. stb_tac. auto. }
-      hcall (_, _) _ with "".
-      { iModIntro. iSplits;ss. }
-      { oauto. } mDesAll. des.
-      steps.
-      rewrite decomp_ret. unfold _sreturn_c. steps. resolve_get. resolve_get. steps.
-      unfold sem_xor_c, sem_binarith_c, sem_cast_c. steps. astop. steps. force_l. eexists. steps.
-      hret tt;ss. iModIntro. iSplit;ss. iSplit;ss.
-      iExists (Ptrofs.of_int64 i0).
-      iSplitR "A1";[iSplitR "POST"|];unfold Vptrofs in *;des_ifs_safe;repeat (rewrite Ptrofs.of_int64_to_int64;ss).
-      + unfold Int64.xor, Ptrofs.xor. iPureIntro. f_equal. f_equal. unfold Ptrofs.to_int64. f_equal.
-        do 2 rewrite Int64.unsigned_repr_eq. rewrite Ptrofs.unsigned_repr_eq.
-        replace Ptrofs.modulus with Int64.modulus by auto.
-        set (Ptrofs.unsigned v1) as x. set (Ptrofs.unsigned (Ptrofs.add i a)) as y.
-        admit "".
-      + iExists _, _. iSplits;[..|iApply "POST"];ss.
-      + iExists _. iSplits;ss.
-        Unshelve. et. 
-  Qed.
+  Admitted.
 
-  Lemma sim_insert (sk: alist string Sk.gdef) :
+  Require Import ClightDmExprgen.
+  From compcertip Require Import Clight.
+
+  Lemma unfold_expr sk ce' e le expr :
+    (eval_expr_c sk ce' e le expr : itree Es val)
+    =
+    match expr with
+    | Econst_int i ty => Ret (Vint i)
+    | Econst_float f ty => Ret (Vfloat f)
+    | Econst_single f ty => Ret (Vsingle f)
+    | Econst_long i ty => Ret (Vlong i)
+    | Etempvar id ty => (alist_find (string_of_ident id) le)?
+    | Eaddrof a ty =>
+      _eval_lvalue_c sk ce' e (eval_expr_c sk ce' e le) a
+    | Eunop op a ty =>
+      v <- eval_expr_c sk ce' e le a;;
+      unary_op_c op v (Clight.typeof a)
+    | Ebinop op a1 a2 ty =>
+      v1 <- eval_expr_c sk ce' e le a1;;
+      v2 <- eval_expr_c sk ce' e le a2;;
+      binary_op_c ce' op
+        v1 (Clight.typeof a1)
+        v2 (Clight.typeof a2)
+    | Ecast a ty =>
+      v <- eval_expr_c sk ce' e le a;;
+      sem_cast_c v (Clight.typeof a) ty
+    | Esizeof ty1 ty =>
+      Ret (Vptrofs (Ptrofs.repr (sizeof ce' ty1)))
+    | Ealignof ty1 ty =>
+      Ret (Vptrofs (Ptrofs.repr (alignof ce' ty1)))
+    | a =>
+      vp <- _eval_lvalue_c sk ce' e (eval_expr_c sk ce' e le) a;;
+      v <- deref_loc_c (Clight.typeof a) vp;; Ret v
+    end.
+  Proof. des_ifs. Qed.
+
+  Lemma isim_ccallU_malloc
+        o stb fuel1
+        R_src R_tgt
+        (Q: Any.t -> Any.t -> R_src -> R_tgt -> iProp)
+        I r g f_src f_tgt st_src st_tgt
+        (arg: list val) itr_src (ktr_tgt: val -> _)
+        fuel0
+        (STBINCL': stb_incl (to_stb MemStb) stb)
+        (DEPTH: ord_lt (ord_pure 0%nat) o)
+        (FUEL: Ord.lt fuel1 fuel0)
+    :
+      bi_entails
+        (∃ b ofs, isim (world:=unit) top2 I "xorlist" stb o (g, g, true, true) Q None (st_src, itr_src) (st_tgt, ktr_tgt (Vptr b ofs)))
+        (isim (world:=unit) top2 I "xorlist" stb o (r, g, f_src, f_tgt) Q None (st_src, itr_src) (st_tgt, ccallU "malloc" arg >>= ktr_tgt)).
+  Proof. Admitted.
+
+  Lemma isim_ccallU_load2
+        o stb fuel1
+        R_src R_tgt
+        (Q: Any.t -> Any.t -> R_src -> R_tgt -> iProp)
+        I r g f_src f_tgt st_src st_tgt
+        (arg: memory_chunk * val) itr_src (ktr_tgt: val -> _)
+        fuel0
+        (STBINCL': stb_incl (to_stb MemStb) stb)
+        (DEPTH: ord_lt (ord_pure 0%nat) o)
+        (FUEL: Ord.lt fuel1 fuel0)
+    :
+      bi_entails
+        (∃ b ofs, isim (world:=unit) top2 I "xorlist" stb o (g, g, true, true) Q None (st_src, itr_src) (st_tgt, ktr_tgt (Vptr b ofs)))
+        (isim (world:=unit) top2 I "xorlist" stb o (r, g, f_src, f_tgt) Q None (st_src, itr_src) (st_tgt, ccallU "load" arg >>= ktr_tgt)).
+  Proof. Admitted.
+
+  Lemma isim_ccallU_store2
+        o stb fuel1
+        R_src R_tgt
+        (Q: Any.t -> Any.t -> R_src -> R_tgt -> iProp)
+        I r g f_src f_tgt st_src st_tgt
+        (arg: memory_chunk * val * val) itr_src (ktr_tgt: val -> _)
+        fuel0
+        (STBINCL': stb_incl (to_stb MemStb) stb)
+        (DEPTH: ord_lt (ord_pure 0%nat) o)
+        (FUEL: Ord.lt fuel1 fuel0)
+    :
+      bi_entails
+        (∃ b ofs, isim (world:=unit) top2 I "xorlist" stb o (g, g, true, true) Q None (st_src, itr_src) (st_tgt, ktr_tgt (Vptr b ofs)))
+        (isim (world:=unit) top2 I "xorlist" stb o (r, g, f_src, f_tgt) Q None (st_src, itr_src) (st_tgt, ccallU "store" arg >>= ktr_tgt)).
+  Proof. Admitted.
+
+  Lemma decomp_se sk ce' retty s1 s2 e le
+  :
+    (decomp_stmt sk ce' retty (Clight.Ssequence s1 s2) e le : itree Es runtime_env)
+    = '(e', le', bc, v) <- (tau;; decomp_stmt sk ce' retty s1 e le);;
+      match v with
+      | Some retval =>
+        Ret (e', le', None, v)
+      | None =>
+        match bc with
+        | None =>
+          tau;; decomp_stmt sk ce' retty s2 e' le'
+        | Some true =>
+          tau;; Ret (e', le', bc, None)
+        | Some false =>
+          tau;; Ret (e', le', bc, None)
+        end
+      end.
+  Proof. ss. Qed.
+       
+  Lemma sim_insert (sk: Sk.t) :
     sim_fnsem wf top2
-      ("insert",
-        fun_to_tgt (SModSem.mn (SMod.get_modsem Sxor sk)) (GlobalStb sk)
-                   {| fsb_fspec := insert_spec; fsb_body := λ _ : option string * Any.t, triggerNB |})
-      ("insert", cfunU insert_body).
+      ("add", fun_to_tgt "xorlist" (GlobalStb sk) (mk_pure add_spec))
+      ("add", cfunU (decomp_func sk ce f_add)).
   Proof.
-  Opaque Maps.PTree.set.
-  Opaque Maps.PTree.get.
-  Opaque decomp_stmt.
-    init. harg. destruct x as [[[[[[v_head v_tail] p_head] p_tail] item] from_tail] xs].
-    mDesAll. des. steps.
-    unfold function_entry_c. steps. resolve_seq.
+    Opaque repr_to.
+    Opaque allocated_with.
+    Opaque points_to.
+    Opaque ccallU.
+    Opaque free_list_aux.
+    Opaque ClightDmgen.blocks_of_env.
+    Opaque _sassign_c.
+    Opaque _sreturn_c.
+    Opaque _eval_lvalue_c.
+    Opaque _scall_c.
+    Opaque ClightDmExprgen.eval_expr_c.
+    init. harg.
+    unfold decomp_func, function_entry_c.
+    Opaque decomp_stmt.
+    ss. des_ifs_safe. mDesAll. clarify.
+    steps.
+    repeat rewrite decomp_se. steps.
+    hide_k.
 
-    rewrite decomp_call. unfold _scall_c. prep.
-    repeat (repeat (rewrite Maps.PTree.gso;[|solve [auto]])
-            ;first [rewrite Maps.PTree.gss|rewrite Maps.PTree.gempty|use_get]).
-    unfold Globalenvs.Genv.find_symbol.
-    Compute (length xorlist.global_definitions).
-    replace (Maps.PTree.get xorlist._malloc _) with (Some 57%positive) by auto. steps.
-    Transparent Globalenvs.Genv.find_funct_ptr Globalenvs.Genv.find_def fold_left Globalenvs.Genv.add_global Ctypes.prog_defs xorlist.prog Globalenvs.Genv.empty_genv Ctypes.prog_public. unfold Globalenvs.Genv.find_funct_ptr, Globalenvs.Genv.find_def in Heq.
-    unfold xorlist.prog in Heq. unfold Clightdefs.mkprogram, Clightdefs.build_composite_env' in Heq.
-    unfold build_composite_env in Heq. unfold add_composite_definitions in Heq. unfold xorlist.composites in Heq.
-    unfold composite_of_def in Heq. Transparent Maps.PTree.get Maps.PTree.set. simpl in Heq. simpl in Heq1. Transparent xorlist.__Node. simpl in Heq1. unfold "cSet" in Heq1.
-    Maps.PTree.set = 
-λ (A : Type) (p : positive) (x : A) (m : Maps.PTree.tree A),
-  match m with
-  | Maps.PTree.Empty => Maps.PTree.Nodes (Maps.PTree.set0 p x)
-  | Maps.PTree.Nodes m' => Maps.PTree.Nodes (Maps.PTree.set' p x m')
-  end
-PTree.set = 
-fix set (A : Type) (i : positive) (v : A) (m : PTree.t A) {struct i} : PTree.t A :=
-  match m with
-  | PTree.Leaf =>
-      match i with
-      | (ii~1)%positive => PTree.Node PTree.Leaf None (set A ii v PTree.Leaf)
-      | (ii~0)%positive => PTree.Node (set A ii v PTree.Leaf) None PTree.Leaf
-      | 1%positive => PTree.Node PTree.Leaf (Some v) PTree.Leaf
-      end
-  | PTree.Node l o r =>
-      match i with
-      | (ii~1)%positive => PTree.Node l o (set A ii v r)
-      | (ii~0)%positive => PTree.Node (set A ii v l) o r
-      | 1%positive => PTree.Node l (Some v) r
-      end
-  end
-    (* former one is newer *)
-    Opaque Maps.PTree.get Maps.PTree.set.
+    rewrite decomp_seq.
+    Transparent decomp_stmt. steps.
+
+    set (decomp_stmt _ _).
+    Red.prw _red_gen 1 1 0.
+    steps.
+    hide_k. 
+    steps. unhide_k.
     
-    (* rewrite gempty is not working *)
-    unfold sem_cast_c. steps.
+    steps.
+    ss. clarify. rewrite Any.upcast_downcast. ss.
+    econs; ss. red.
+    apply isim_fun_to_tgt; auto. i; ss.
+    unfold decomp_func, function_entry_c. ss.
+    iIntros "[INV PRE]". des_ifs_safe. ss.
+    iDestruct "PRE" as "[PRE %]".
+    iDestruct "PRE" as (hd_old tl_old) "[[[% HD] TL] XOR]".
+    ss. clarify. rewrite Any.upcast_downcast. ss.
+    rewrite bind_ret_l. rewrite bind_ret_l. 
+    ss. rewrite bind_ret_l. rewrite bind_ret_l.
+    rewrite bind_bind. rewrite bind_bind. 
+    rewrite bind_tau. iApply isim_tau_tgt. rewrite bind_tau.
+    rewrite bind_tau.
+    iApply isim_tau_tgt. unfold _scall_c.
+    rewrite bind_bind. rewrite bind_bind.
+    unfold Cop.classify_fun. unfold Clight.typeof.
+    rewrite bind_tau. iApply isim_tau_tgt.
+    rewrite bind_bind.
+    rewrite unfold_expr.
+    unfold _eval_lvalue_c.
+    assert (exists i, SkEnv.id2blk (Sk.load_skenv sk) (string_of_ident _malloc) = Some i).
+    { admit "". }
+    des. rewrite H3.
+    replace (alist_find _ _) with (@None (Values.block * type)) by refl.
+    rewrite bind_ret_l. unfold deref_loc_c.
+    unfold access_mode. unfold typeof. rewrite bind_ret_l.
+    rewrite bind_ret_l. unfold eval_exprlist_c.
+    rewrite unfold_expr. set (sizeof _ _).
+    unfold ce in z. simpl in z. unfold prog in z.
+    unfold mkprogram in z. destruct (build_composite_env' _ _) in z.
+    simpl in z. 
+    Transparent prog_comp_env.
+    unfold prog_comp_env in z. unfold build_composite_env in e.
+    unfold composites in e.
+    simpl in e. clarify. simpl in z.
+    assert (z = 16) by refl. rewrite H4.
+    do 2 rewrite bind_ret_l. unfold sem_cast_c.
+    unfold Cop.classify_cast. unfold tulong. unfold typeof.
+    destruct Archi.ptr64; clarify.
+    destruct (Vptrofs _) eqn: E; clarify.
+    do 2 rewrite bind_ret_l.
+    destruct (Ptrofs.eq_dec _ _); clarify.
+    assert (SkEnv.blk2id (Sk.load_skenv sk) i = Some (string_of_ident _malloc)). 
+    { admit "". }
+    replace (Init.Nat.pred _) with i by nia.
+    assert (alist_find (string_of_ident _malloc) sk = alist_find (string_of_ident _malloc) xorlist0.xor.(Mod.sk)).
+    { admit "". }
+    Transparent get_sk.
+    Transparent alist_find.
+    simpl in H6. 
+    Opaque alist_find.
+    set (Gfun _) in H6.
+    assert (nth_error sk i = Some (string_of_ident _malloc, g↑)).
+    { admit "". }
+    rewrite H7. unfold unwrapU. rewrite bind_ret_l.
+    rewrite Any.upcast_downcast. rewrite bind_ret_l.
+    unfold g. rewrite bind_ret_l. unfold type_of_fundef.
+    destruct (type_eq _ _); clarify.
+    Opaque alist_remove.
+    iApply isim_ccallU_malloc.
+    1,2,3:admit "".
+    iExists xH, Ptrofs.zero.
+    rewrite bind_ret_l.
+    do 2 rewrite bind_tau. do 2 iApply isim_tau_tgt.
+    rewrite bind_bind. rewrite bind_bind.
+    hide_k.
+    rewrite bind_ret_l. rewrite bind_ret_l.
+    rewrite bind_ret_l. do 5 rewrite bind_tau.
+    do 3 iApply isim_tau_tgt.
+    destruct ("hd_handler" ?[ eq ] "entry") eqn: E2; clarify.
+    unfold is_ptr_val. do 3 rewrite bind_bind.
+    destruct (_ "hd_handler" _).
+    2:{ admit "". }
+    rewrite bind_ret_l.
+    destruct v3. 1,2,3,4,5: admit "".
+    rewrite bind_ret_l.
+    unfold tptr. rewrite bind_ret_r.
+    iApply isim_ccallU_load2.
+    1,2,3:admit "".
+    iExists xH, Ptrofs.zero.
+    rewrite bind_ret_l.
+    do 5 rewrite bind_tau. do 3 iApply isim_tau_tgt.
+    do 4 rewrite bind_bind.
+    destruct ("tl_handler" ?[ eq ] "hd") eqn: E3; clarify.
+    destruct (alist_find _ _).
+    rewrite bind_bind.
+    rewrite bind_ret_l.
+    rewrite bind_bind.
+    iApply isim_ccallU_load2.
+    1,2,3:admit "".
+    unfold tptr. rewrite bind_ret_r.
+    do 2 rewrite bind_bind. 
 
-    astart 2. unfold ccallU. steps. acatch. { apply MEMINCL. stb_tac. auto. }
-    hcall (_, _) _ with "".
-    { iModIntro. iSplits;ss.  }
+    ss.
+    ss.
+    unfold alist_remove. 
+    unfold type_eq.
+    
+     clear. clearbody ce.
+    hred_r. 
+
+    hred_r.
+
+    des_ifs_safe.
+    hred_r.
+
+    set (eval_expr_c _ _ _ _ _) as t.
+    Set Printing All.
+
+
+    unfold ClightDmExprgen.eval_expr_c.
+    destruct (Cop.classify_fun _).
+     ss.
+     hred_r. iApply isim_tau_tgt. hred_r. iApply isim_tau_tgt.
+    ss. hred_r. des_ifs_safe.
+    iApply isim_apc. iExists (Some (2%nat : Ord.t)).
+    iPoseProof (val_multimap with "PTR1") as "%".
+    iPoseProof (val_multimap with "PTR2") as "%".
+    - des_ifs_safe. hred_r. iApply isim_ccallU_capture2; ss; oauto.
   Admitted.
  
   Lemma sim_delete (sk: alist string Sk.gdef) :
