clightdm/proofmode/CIProofMode.v
@@ -1,0 +1,240 @@
+Require Import Coqlib.
+Require Import Any.
+Require Import ModSem.
+Require Import PCM IPM.
+Require Import HoareDef STB.
+Require Export HSim IProofMode.
+Require Import ClightDmMem1.
+From compcertip Require Import AST Values Integers Memdata.
+
+Section MEM.
+
+  Context `{@GRA.inG memcntRA Σ}.
+  Context `{@GRA.inG memphyRA Σ}.
+  Context `{@GRA.inG memhdRA Σ}.
+  Context `{@GRA.inG memidRA Σ}.
+  Variable world: Type.
+  Variable le: relation world.
+  Variable I: world -> Any.t -> Any.t -> iProp.
+
+  Variable mn: mname.
+
+  Lemma isim_ccallU_salloc
+        o stb w0 fuel1
+        R_src R_tgt
+        (Q: Any.t -> Any.t -> R_src -> R_tgt -> iProp)
+        r g f_src f_tgt st_src st_tgt
+        sz itr_src (ktr_tgt: block -> _)
+        fuel0
+        (STBINCL: stb_incl (to_stb MemStb) stb)
+        (DEPTH: ord_lt (ord_pure 0%nat) o)
+        (FUEL: Ord.lt fuel1 fuel0)
+    :
+      bi_entails
+        (inv_with le I w0 st_src st_tgt
+                  **
+                  (∀ st_src st_tgt vaddr b,
+                      ((inv_with le I w0 st_src st_tgt) ** (vaddr |-1#> List.repeat Undef (Z.to_nat sz) ** vaddr ⊸ (b, 0) ** b ↱1# (sz, Local, None))) -* isim le I mn stb o (g, g, true, true) Q (Some fuel1) (st_src, itr_src) (st_tgt, ktr_tgt b)))
+        (isim le I mn stb o (r, g, f_src, f_tgt) Q (Some fuel0) (st_src, itr_src) (st_tgt, ccallU "salloc" sz >>= ktr_tgt)).
+  Proof.
+    iIntros "[H0 H1]". iApply isim_ccallU_pure; et.
+    { eapply fn_has_spec_in_stb; et.
+      { eapply STBINCL. stb_tac. ss. }
+      { ss. }
+      { ss. } }
+    instantiate (1:=sz).
+    ss.
+    iSplitL "H0".
+    { iSplit; ss. }
+    iIntros (st_src0 st_tgt0 ret_src ret_tgt) "H0".
+    iDestruct "H0" as "[INV [RES %]]".
+    iDestruct "RES" as (b vaddr) "[[[% STR] LIV] PTR]".
+    des. clarify.
+    iExists _. iSplit; ss.
+    iApply "H1". iFrame. 
+  Qed.
+
+  Lemma isim_ccallU_sfree
+        o stb w0 fuel1
+        R_src R_tgt
+        (Q: Any.t -> Any.t -> R_src -> R_tgt -> iProp)
+        r g f_src f_tgt st_src st_tgt
+        mvl vaddr b sz opti itr_src (ktr_tgt: unit -> _)
+        fuel0
+        (STBINCL: stb_incl (to_stb MemStb) stb)
+        (DEPTH: ord_lt (ord_pure 0%nat) o)
+        (FUEL: Ord.lt fuel1 fuel0)
+    :
+      bi_entails
+        (inv_with le I w0 st_src st_tgt
+                  ** (vaddr |-1#> mvl ** vaddr ⊸ (b, 0) ** b ↱1# (sz, Local, opti) ** ⌜Z.of_nat (List.length mvl) = sz⌝)
+                  **
+                  (∀ st_src st_tgt,
+                      ((inv_with le I w0 st_src st_tgt)) -* isim le I mn stb o (g, g, true, true) Q (Some fuel1) (st_src, itr_src) (st_tgt, ktr_tgt tt)))
+        (isim le I mn stb o (r, g, f_src, f_tgt) Q (Some fuel0) (st_src, itr_src) (st_tgt, ccallU "sfree" (b, sz) >>= ktr_tgt)).
+  Proof.
+    iIntros "[H0 H1]". iApply isim_ccallU_pure; et.
+    { eapply fn_has_spec_in_stb; et.
+      { eapply STBINCL. stb_tac. ss. }
+      { ss. des_ifs. }
+      { ss. des_ifs. } }
+    instantiate (1:=()).
+    ss.
+    iSplitL "H0".
+    { iDestruct "H0" as "[INV PRE]". iFrame. iSplit; ss.
+      iDestruct "PRE" as "[[[STR PTR] LIV] %]". iExists _, _, _, _, _.
+      iFrame. ss. }
+    iIntros (st_src0 st_tgt0 ret_src ret_tgt) "H0".
+    iDestruct "H0" as "[INV [% %]]".
+    des. clarify.
+    iExists _. iSplit; ss.
+    iApply "H1". iFrame. 
+  Qed.
+
+  Lemma isim_ccallU_load
+        o stb w0 fuel1
+        R_src R_tgt
+        (Q: Any.t -> Any.t -> R_src -> R_tgt -> iProp)
+        r g f_src f_tgt st_src st_tgt
+        chunk vaddr q mvs itr_src (ktr_tgt: val -> _)
+        fuel0
+        (STBINCL: stb_incl (to_stb MemStb) stb)
+        (DEPTH: ord_lt (ord_pure 0%nat) o)
+        (FUEL: Ord.lt fuel1 fuel0)
+    :
+      bi_entails
+        (inv_with le I w0 st_src st_tgt
+                  ** (vaddr |-q#> mvs)
+                  **
+                  (∀ st_src st_tgt,
+                      ((inv_with le I w0 st_src st_tgt) ** (vaddr |-q#> mvs)) -* isim le I mn stb o (g, g, true, true) Q (Some fuel1) (st_src, itr_src) (st_tgt, ktr_tgt (decode_val chunk mvs))))
+        (isim le I mn stb o (r, g, f_src, f_tgt) Q (Some fuel0) (st_src, itr_src) (st_tgt, ccallU "load" (chunk, vaddr) >>= ktr_tgt)).
+  Proof.
+    iIntros "[H0 H1]". iApply isim_ccallU_pure; et.
+    { eapply fn_has_spec_in_stb; et.
+      { eapply STBINCL. stb_tac. ss. }
+      { ss. des_ifs_safe. destruct p0. ss. }
+      { ss. des_ifs_safe. destruct p0. ss. } }
+    instantiate (1:=(chunk, vaddr, q, mvs)).
+    ss.
+    iSplitL "H0".
+    { iDestruct "H0" as "[INV PRE]". iSplitL "INV"; et. }
+    iIntros (st_src0 st_tgt0 ret_src ret_tgt) "H0".
+    iDestruct "H0" as "[INV [RES %]]".
+    iDestruct "RES" as (v) "[% POST]".
+    des. clarify.
+    iExists _. iSplit; ss.
+    iApply "H1". iFrame. 
+  Qed.
+
+  Lemma isim_ccallU_store
+        o stb w0 fuel1
+        R_src R_tgt
+        (Q: Any.t -> Any.t -> R_src -> R_tgt -> iProp)
+        r g f_src f_tgt st_src st_tgt
+        chunk vaddr v_new itr_src (ktr_tgt: unit -> _)
+        fuel0
+        (STBINCL: stb_incl (to_stb MemStb) stb)
+        (DEPTH: ord_lt (ord_pure 0%nat) o)
+        (FUEL: Ord.lt fuel1 fuel0)
+    :
+      bi_entails
+        (inv_with le I w0 st_src st_tgt
+                  ** (∃ mvs_old, ⌜length mvs_old = size_chunk_nat chunk⌝ ** vaddr |-1#> mvs_old)
+                  **
+                  (∀ st_src st_tgt,
+                      ((inv_with le I w0 st_src st_tgt) ** (vaddr |-1#> (encode_val chunk v_new))) -* isim le I mn stb o (g, g, true, true) Q (Some fuel1) (st_src, itr_src) (st_tgt, ktr_tgt tt)))
+        (isim le I mn stb o (r, g, f_src, f_tgt) Q (Some fuel0) (st_src, itr_src) (st_tgt, ccallU "store" (chunk, vaddr, v_new) >>= ktr_tgt)).
+  Proof.
+    iIntros "[H0 H1]". iApply isim_ccallU_pure; et.
+    { eapply fn_has_spec_in_stb; et.
+      { eapply STBINCL. stb_tac. ss. }
+      { ss. des_ifs_safe. destruct p. ss. }
+      { ss. des_ifs_safe. destruct p. ss. } }
+    instantiate (1:=(chunk, vaddr, v_new)).
+    ss.
+    iSplitL "H0".
+    { iDestruct "H0" as "[INV PRE]". iFrame. iSplit; ss.
+      iDestruct "PRE" as (mvs_old) "[% PRE]". iExists _. iSplit; ss. }
+    iIntros (st_src0 st_tgt0 ret_src ret_tgt) "H0".
+    iDestruct "H0" as "[INV [RES %]]".
+    iDestruct "RES" as (v) "[% POST]".
+    des. clarify.
+    iExists _. iSplit; ss.
+    iApply "H1". iFrame. 
+  Qed.
+
+  
+  Lemma isim_ccallU_capture1
+        o stb w0 fuel1
+        R_src R_tgt
+        (Q: Any.t -> Any.t -> R_src -> R_tgt -> iProp)
+        r g f_src f_tgt st_src st_tgt
+        i itr_src (ktr_tgt: val -> _)
+        fuel0
+        (STBINCL: stb_incl (to_stb MemStb) stb)
+        (DEPTH: ord_lt (ord_pure 0%nat) o)
+        (FUEL: Ord.lt fuel1 fuel0)
+    :
+      bi_entails
+        (inv_with le I w0 st_src st_tgt
+                  **
+                  (∀ st_src st_tgt,
+                      ((inv_with le I w0 st_src st_tgt)) -* isim le I mn stb o (g, g, true, true) Q (Some fuel1) (st_src, itr_src) (st_tgt, ktr_tgt (Vptrofs i))))
+        (isim le I mn stb o (r, g, f_src, f_tgt) Q (Some fuel0) (st_src, itr_src) (st_tgt, ccallU "capture" [Vptrofs i] >>= ktr_tgt)).
+  Proof.
+    iIntros "[H0 H1]". iApply isim_ccallU_pure; et.
+    { eapply fn_has_spec_in_stb; et.
+      { eapply STBINCL. stb_tac. ss. }
+      { instantiate (1:= inl _). ss. }
+      { ss. } }
+    instantiate (1:=(i)).
+    ss.
+    iSplitL "H0".
+    { iSplit; ss. }
+    iIntros (st_src0 st_tgt0 ret_src ret_tgt) "H0".
+    iDestruct "H0" as "[INV [% %]]".
+    des. clarify.
+    iExists _. iSplit; ss.
+    iApply "H1". iFrame.
+  Qed.
+
+  Lemma isim_ccallU_capture2
+        o stb w0 fuel1
+        R_src R_tgt
+        (Q: Any.t -> Any.t -> R_src -> R_tgt -> iProp)
+        r g f_src f_tgt st_src st_tgt
+        b ofs q sz tg opti itr_src (ktr_tgt: val -> _)
+        fuel0
+        (STBINCL: stb_incl (to_stb MemStb) stb)
+        (DEPTH: ord_lt (ord_pure 0%nat) o)
+        (FUEL: Ord.lt fuel1 fuel0)
+    :
+      bi_entails
+        (inv_with le I w0 st_src st_tgt
+                  ** b ↱q# (sz, tg, opti)
+                  **
+                  (∀ st_src st_tgt ret,
+                      ((inv_with le I w0 st_src st_tgt) ** (∃ i, ⌜ret = (Vptrofs (Ptrofs.add i ofs))⌝ ** b ↱q# (sz, tg, Some (Ptrofs.unsigned i)))) -* isim le I mn stb o (g, g, true, true) Q (Some fuel1) (st_src, itr_src) (st_tgt, ktr_tgt ret)))
+        (isim le I mn stb o (r, g, f_src, f_tgt) Q (Some fuel0) (st_src, itr_src) (st_tgt, ccallU "capture" [Vptr b ofs] >>= ktr_tgt)).
+  Proof.
+    iIntros "[H0 H1]". iApply isim_ccallU_pure; et.
+    { eapply fn_has_spec_in_stb; et.
+      { eapply STBINCL. stb_tac. ss. }
+      { ss. instantiate (1:= inr _).
+        ss. unfold capture_hoare2. des_ifs_safe. destruct p. ss. }
+      { ss. unfold capture_hoare2. des_ifs_safe. destruct p. ss. } }
+    instantiate (1:=(b, ofs, q, sz, tg)).
+    ss.
+    iSplitL "H0".
+    { iDestruct "H0" as "[INV PRE]". iSplitL "INV"; et. }
+    iIntros (st_src0 st_tgt0 ret_src ret_tgt) "H0".
+    iDestruct "H0" as "[INV [RES %]]".
+    iDestruct "RES" as (v) "[% POST]".
+    des. clarify.
+    iExists _. iSplit; ss.
+    iApply "H1". iSplitL "INV"; iFrame.
+    iExists _. iSplit; ss.
+  Qed.
+
+End MEM.
